%%% Exercise 1.4.11
\begin{exrc}[11]
    Show that if \(u(x, t) = (f * H_t)(x)\) where \(H_t\) is the heat kernel,
    and \(f\) is Riemann integrable, then
    \begin{equation*}
        \int_{0}^{1} |u(x, t) - f(x)|^2 \ud x \to 0 \quad \text{as \(t \to 0\)}.
    \end{equation*}

\begin{soln}
    By Parseval's identity,
    \begin{equation*}
        \int_{0}^{1} |u(x, t) - f(x)| \ud x
        = \sum_{n = -\infty}^{\infty} |\hat{f}(n) e^{-4 \pi^2 n^2 t} - \hat{f}(n)|
        = \sum_{n = -\infty}^{\infty} |\hat{f}(n)| |e^{-4 \pi^2 n^2 t} - 1|.
    \end{equation*}
    Since \(f\) is Riemann integrable, we know \(\hat{f}(n) = o(1)\).
    Hence, since \(|e^{-4 \pi^2 n^2 t} - 1| \leq 2\) when \(t > 0\),
    we can find an \(N\) such that
    \begin{equation*}
        \sum_{|n| \geq N}^{} |\hat{f}(n)| |e^{-4 \pi^2 n^2 t} - 1| < 2\epsilon.
    \end{equation*}
    Then noting the since the Fourier coefficients of a (Riemann) integrable
    function are bounded, for small enough \(t > 0\), we have
    \begin{equation*}
        \sum_{|n| < N}^{} |\hat{f}(n)| |e^{-4 \pi^2 n^2 t} - 1| < \epsilon.
    \end{equation*}
    Therefore, the sum converges, hence \(u(x, t) - f(x) \to 0\) in the mean square sense.

\end{soln}
\end{exrc}
