%%% Exercise 1.2.6
\begin{exrc}[6]
    Let \(f\) be the function defined on \([-\pi, \pi]\) by \(f(\theta) = |\theta|\).
    \begin{enumerate}[(a)]
    \item
        Draw the graph of \(f\).
    \item
        Calculate the Fourier coefficients of \(f\), and show that
        \begin{equation*}
            \hat{f}(n) = 
            \begin{cases}
                \frac{\pi}{2} & \text{if \(n = 0\)},\\
                \frac{-1 + (-1)^n}{\pi n^2} & \text{if \(n \neq 0\)}.
            \end{cases}
        \end{equation*}
    \item
        What is the Fourier series of \(f\) in terms of sines and cosines?
    \item
        Taking \(\theta = 0\), prove that
        \begin{equation*}
            \sum_{n \text{ odd } \geq 1}^{} \frac{1}{n^2} = \frac{\pi^2}{8}
            \quad \text{and} \quad
            \sum_{n = 1}^{\infty} \frac{1}{n^2}= \frac{\pi^2}{6}.
        \end{equation*}
    \end{enumerate}

\begin{soln}
    \begin{enumerate}[(a)]
    \item
        The following is a graph of \(f(\theta)\) extended periodically to \([-2\pi, 2\pi]\).

        \begin{tikzpicture}
        \begin{axis}[
            axis lines = left,
            xlabel = \(x\),
            ylabel = {\(f(\theta)\)},
            xmin=-2*pi - 0.5,
            xmax=2*pi + 0.5,
            xtick={-2*pi, -(3/2)*pi, -pi, -(1/2)*pi, 0, (1/2)*pi, pi, (3/2)*pi, 2*pi},
            xticklabels={$-2\pi$,,$-\pi$,,0,,$\pi$,,$2\pi$},
            ymax = pi + 0.25,
            ytick={0, pi},
            yticklabels={0,$\pi$},
        ]
        \addplot [
            domain=-pi:pi,
            samples=101, 
        ]
        {abs(x)};
        \addlegendentry{\(f(\theta)\)}
        \addplot [
            domain=-2 * pi:-pi,
            samples=100, 
        ]
        {x + 2 * pi};
        \addplot [
            domain=pi:2*pi,
            samples=100, 
        ]
        {-x + 2 * pi};

        \end{axis}
        \end{tikzpicture}

    \item
        Note that \(f\) is an even function,
        so by exercise 2, \(\hat{f}(n) = \frac{1}{\pi}\int_{0}^{\pi} f(0) \cos n\theta  \ud \theta\).
        Calculation yields
        \begin{equation*}
            \hat{f}(0) = \frac{1}{2\pi} \int_{-\pi}^{\pi} f(\theta) \ud \theta
            = \frac{1}{\pi} \int_{0}^{\pi} \theta \ud \theta
            = \frac{1}{\pi} \frac{\pi^2}{2}
            = \frac{\pi}{2}.
        \end{equation*}
        and
        \begin{equation*}
            \hat{f}(n)
            = \frac{1}{\pi} \int_{0}^{\pi} \theta \cos n\theta \ud \theta
            = \frac{\pi \sin n\pi}{\pi n} - \frac{1}{n\pi} \int_{0}^{\pi} \sin n\theta \ud \theta
            = 0 + \frac{{(-1)}^n - 1}{\pi n^2}
        \end{equation*}
        for \(n \neq 0\).
    \item
        Since \(f\) is even, by exercise 2, the Fourier series of \(f\) is a cosine series with
        \begin{equation*}
            f(\theta) \sim \hat{f}(0) + \sum_{n = 1}^{\infty} (\hat{f}(n) + \hat{f}(-n)) \cos n\theta
            = \frac{\pi}{2} + 2\sum_{n = 1}^{\infty} \frac{-1 - {(-1)}^n}{\pi n^2} \cos n\theta.
        \end{equation*}
        Note that the Fourier series of \(f\) converges to \(f\) since \(\hat{f}(n) = O(1 / n^2)\),
        so equality holds above.
        Also, note that the Fourier coefficients are zero whenever \(n\) is nonzero even, so
        \begin{equation*}
            f(\theta) = \frac{\pi}{2} + \sum_{n \text{ odd } \geq 1}^{} \frac{4}{\pi n^2} \cos n\theta.
        \end{equation*}
    \item
        By part (c),
        \begin{equation*}
            0 = f(0) = \frac{\pi}{2} + \frac{4}{\pi}\sum_{n \text{ odd } \geq 1}^{} \frac{1}{n^2}
        \end{equation*}
        Solving for the summation yields \(\sum_{n \text{ odd } \geq 1}^{} 1 / n^2 = \pi^2 / 8\).

        Next, note that
        \begin{equation*}
            \sum_{n = 1}^{\infty} \frac{1}{n^2} 
            = \sum_{n \text{ odd } \geq 1}^{} \frac{1}{n^2} + \sum_{n \text{ even } \geq 1}^{} \frac{1}{n^2}
            = \sum_{n = 1}^{\infty} \frac{1}{(2n - 1)^2} + \frac{1}{4} \sum_{n = 1}^{\infty} \frac{1}{n^2}.
        \end{equation*}
        Therefore,
        \begin{equation*}
            \frac{3}{4} \sum_{n = 1}^{\infty} \frac{1}{n^2} = \sum_{n \text{ odd } \geq 1}^{} \frac{1}{n^2}
            = \frac{\pi^2}{8}.
        \end{equation*}
        Hence \(\sum_{}^{} 1 / n^2 = \pi^2 / 6\).
    \end{enumerate}

\end{soln}
\end{exrc}
