%%% Exercise 1.2.17
\begin{exrc}[17]
    An integrable function is said to have a \emph{jump discontinuity} at \(\theta\)
    if the two limits
    \begin{equation*}
        \lim_{h \to 0} f(\theta + h) = f(\theta^+) \quad \text{and} \quad
        \lim_{h \to 0} f(\theta - h) = f(\theta^-) \quad h > 0
    \end{equation*}
    exist.

    \begin{enumerate}[(a)]
    \item
        Prove that if \(f\) has a jump discontinuity at \(\theta\), then
        \begin{equation*}
            \lim_{r \to 1} A_r(f)(\theta) = \frac{f(\theta^+) + f(\theta^-)}{2},
            \quad \text{with \(0 \leq r < 1\)}.
        \end{equation*}
    
    \item
        Show that if \(f\) has a jump discontinuity at \(\theta\),
        the Fourier series of \(f\) at \(\theta\) is Cesàro summable
        to \(\frac{f(\theta^+) + f(\theta^-)}{2}\).
        
    \end{enumerate}

\begin{soln}
    Let \(K_n\) be a good kernel such that
    \begin{equation*}
        \frac{1}{2\pi} \int_{0}^{\pi} K_n(x) \ud x
        = \frac{1}{2\pi} \int_{-\pi}^{0} K_n(x) \ud x
        = \frac{1}{2}.
    \end{equation*}
    Suppose \(f\) is integrable on the circle
    and has a jump continuity at \(x \).
    Then
    \begin{equation*}
        \frac{1}{2\pi} \int_{0}^{\pi} K_n(x) f(x - y) \ud y - \frac{1}{2} f(x^-)
        = \frac{1}{2\pi} \int_{0}^{\pi} K_n(x) [f(x - y) - f(x^-)] \ud x.
    \end{equation*}
    Using the above with almost the exact proof as Theorem 4.1, it can be shown that
    \begin{equation*}
        \abs{\frac{1}{2\pi} \int_{0}^{\pi} K_n(x) f(x - y) \ud y - \frac{1}{2}f(x^-)}
        \to 0
    \end{equation*}
    as \(n \to \infty\).
    Similarly,
    \begin{equation*}
        \abs{\frac{1}{2\pi} \int_{-\pi}^{0} K_n(x) f(x - y) \ud y - \frac{1}{2}f(x^+)}
        \to 0
    \end{equation*}
    as \(n\) becomes large.
    Adding the above two equations shows
    \begin{equation*}
        \abs{(f * K_n)(x) - \frac{f(x^+) - f(x^-)}{2}} \to 0
    \end{equation*}
    as \(n \to \infty\).

    \begin{enumerate}[(a)]
    \item
        Since \(P_r\) is even and a good kernel,
        by our remarks above and the fact that \(A_r(f)(\theta) = (f * P_r)(\theta)\),
        the limit
        \begin{equation*}
            \lim_{r \to 1} A_r(f)(\theta) = \frac{f(\theta^+) - f(\theta^-)}{2}
        \end{equation*}
        holds.
    
    \item
        Similarly, since the Fejér kernel is even and a good kernel,
        by our remarks above and the fact that \(\sigma_N(f)(\theta) = (f * F_N)(x)\),
        the Fourier series of \(f\) at \(\theta\) is Cesàro summable to \(\frac{f(\theta^+)
        + f(\theta^-)}{2}\).

    \end{enumerate}

\end{soln}
\end{exrc}
