%%% Exercise 1.2.1
\begin{exrc}[1]
    Suppose \(f\) is \(2\pi\)-periodic and integrable on any finite interval.
    Prove that if \(a, b \in \R\), then
    \begin{equation*}
        \int_{a}^{b} f(x) \ud x = \int_{a + 2\pi}^{b + 2\pi} f(x) \ud x
        = \int_{a - 2\pi}^{b - 2\pi} f(x) \ud x.
    \end{equation*}
    Also prove that
    \begin{equation*}
        \int_{-\pi}^{\pi} f(x + a) \ud x
        = \int_{-\pi}^{\pi} f(x) \ud x
        = \int_{\pi + a}^{-\pi + a} f(x) \ud x.
    \end{equation*}

\begin{soln}
    For the first set of equalities, since \(f\) is \(2\pi\)-periodic,
    \begin{equation*}
        \int_{a}^{b} f(x) \ud x
        = \int_{a}^{b} f(x + 2\pi) \ud x
        = \int_{a - 2\pi}^{b - 2\pi} f(u) \ud u,
    \end{equation*}
    where \(u = x + 2\pi\).
    Similarly,
    \begin{equation*}
        \int_{a}^{b} f(x) \ud x
        = \int_{a}^{b} f(x - 2\pi) \ud x
        = \int_{a + 2\pi}^{b + 2\pi} f(u) \ud u,
    \end{equation*}
    thus showing the first set of equalities.

    For the other set of equalities, by \(2\pi\)-periodicity, we see
    \begin{align*}
        \int_{-\pi}^{\pi} f(x + a)
        & = \int_{\pi - a}^{-\pi - a} f(x) \\
        & = \int_{-\pi - a}^{-\pi} f(x) + \int_{-\pi}^{\pi - a} f(x) \\
        & = \int_{\pi - a}^{\pi} f(x) + \int_{-\pi}^{\pi - a} f(x) \\
        & = \int_{-\pi}^{\pi} f(x),
    \end{align*}
    where the third equality follows from the first set of equalities proven above.
    The other equality follows by substituting \(a\) for \(-a\) above.

    


     

\end{soln}
\end{exrc}
